Fomega/Basic/Preservation.lean
@@ -9,95 +9,154 @@ import Fomega.Basic.Classification
 
 namespace Fomega.Proof
 
+
+  inductive CtxRed : Ctx -> Ctx -> Prop where
+  | nil : CtxRed [] []
+  | head : A -β> A' -> CtxRed (A::Γ) (A'::Γ)
+  | tail : CtxRed Γ Γ' -> CtxRed (A::Γ) (A::Γ')
+
+  namespace CtxRed
+
+    theorem refl : CtxRed Γ Γ := by
+    induction Γ
+    case _ => constructor
+    case _ hd tl ih => apply tail; apply ih
+
+    theorem nth x : CtxRed Γ Γ' -> Γ d@ x = Γ' d@ x ∨ Γ d@ x -β> Γ' d@ x := by
+    intro j; induction j generalizing x; simp
+    case _ A A' Δ r =>
+      cases x <;> simp
+      apply Or.inr; apply Red.subst1_same; apply r
+    case _ Γ Γ' A _ ih =>
+      cases x <;> simp
+      case _ x =>
+        cases (ih x)
+        case _ h => apply Or.inl; rw [h]
+        case _ h => apply Or.inr; apply Red.subst1_same; apply h
+
+  end CtxRed
+
+  @[simp]
+  abbrev PreservationType (Γ : Ctx) : (v : JudgmentVariant) -> JudgmentIndex v -> Prop
+  | .prf => λ (t, A) => ∀ {t' Γ'}, t = t' ∨ t -β> t' -> CtxRed Γ Γ' -> Γ' ⊢ t' : A
+  | .wf => λ () => ∀ {Γ'}, CtxRed Γ Γ' -> ⊢ Γ'
+
+  theorem preservation1 : Judgment v Γ ix -> PreservationType Γ v ix := by
+  intro j; induction j <;> simp at *
+  case nil =>
+    intro Γ' r
+    cases r; constructor
+  case cons Γ A K j1 j2 ih1 ih2 =>
+    intro Γ' r
+    cases r
+    case _ A' r => constructor; apply j1; apply ih2 (Or.inr r) CtxRed.refl
+    case _ Γ' r => constructor; apply ih1 r; apply ih2 (Or.inl rfl) r
+  case ax Γ j ih =>
+    intro t' Γ' r1 r2
+    cases r1
+    case _ r1 => rw [<-r1]; constructor; apply ih r2
+    case _ r1 => cases r1
+  case var Γ x K T j1 j2 ih =>
+    intro t' Γ' r1 r2
+    cases r1
+    case _ r1 =>
+      rw [<-r1]; apply @Judgment.conv _ _ (Γ' d@ x) _ K
+
+    case _ r1 => cases r1
+  case pi => sorry
+  case lam Γ A K1 K2 B t j1 j2 j3 ih1 ih2 ih3 => sorry
+  case app => sorry
+  case conv => sorry
+
   -- abbrev ctx_red x Γ Γ' := ∀ n, Γ d@ x -β> Γ' d@ x ∧ (n ≠ x -> Γ d@ n = Γ' d@ n)
 
   -- theorem ctx_red_lift : ctx_red x Γ Γ' -> ctx_red (x + 1) (A::Γ) (A::Γ') := by sorry
 
-  theorem preservation_ctx_lift : (∀ n, Γ d@ n -β> Δ d@ n ∨ Γ d@n = Δ d@ n) ->
-    A -β> A' ∨ A = A' ->
-    ∀ n, (A::Γ) d@ n -β> (A'::Δ) d@ n ∨ (A::Γ) d@n = (A'::Δ) d@ n
-  := by sorry
+  -- theorem preservation_ctx_lift : (∀ n, Γ d@ n -β> Δ d@ n ∨ Γ d@n = Δ d@ n) ->
+  --   A -β> A' ∨ A = A' ->
+  --   ∀ n, (A::Γ) d@ n -β> (A'::Δ) d@ n ∨ (A::Γ) d@n = (A'::Δ) d@ n
+  -- := by sorry
 
-  theorem preservation1_term : Γ ⊢ t : A ->
-    (∀ n, Γ d@ n -β> Δ d@ n ∨ Γ d@n = Δ d@ n) ->
-    Δ ⊢ t : A ∧ (∀ t', t -β> t' -> Δ ⊢ t' : A)
-  := by
-  intro j h
-  induction j generalizing Δ
-  case ax Γ f j ih =>
-    apply And.intro
-    case _ =>
-      apply Proof.ax f
-      intro x
-      cases (h x)
-      case _ hx => apply (ih x h).2 _ hx
-      case _ hx => rw [<-hx]; apply (ih x h).1
-    case _ => intro t' r; cases r
-  case var Γ x K j ih =>
-    apply And.intro
-    case _ =>
-      constructor; constructor
-      cases (h x)
-      case _ hx => apply (ih h).2 _ hx
-      case _ hx => rw [<-hx]; apply (ih h).1
-      apply (ih h).1
-      cases (h x)
-      case _ hx =>
-        exists (Δ d@ x); apply And.intro
-        apply Term.Red.refl; apply Term.RedStar.step; apply hx; apply Term.Red.refl
-      case _ hx => rw [hx]; apply Term.RedConv.refl
-    case _ => intro t' r; cases r
-  case pi Γ A K B j1 j2 ih1 ih2 =>
-    apply And.intro
-    case _ =>
-      constructor
-      apply (ih1 h).1
-      apply (@ih2 (A::Δ) (preservation_ctx_lift h (Or.inr rfl))).1
-    case _ => sorry
-  case tpi => sorry
-  case lam Γ A B K t j1 j2 ih1 ih2 =>
-    apply And.intro
-    case _ =>
-      constructor
-      apply (ih1 h).1
-      apply (@ih2 (A::Δ) (preservation_ctx_lift h (Or.inr rfl))).1
-    case _ =>
-      intro t' r
-      cases r
-      case lam_congr1 A' r =>
-        constructor; constructor
-        apply (ih1 h).2 _ (Term.Red.all_congr1 r)
-        apply (@ih2 (A'::Δ) (preservation_ctx_lift h (Or.inl r))).1
-        apply (ih1 h).1
-        exists (.all mf A' B); apply And.intro
-        apply Term.Red.refl
-        apply Term.Red.congr1 (λ A => .all mf A B) Term.Red.all_congr1
-        apply Term.RedStar.step r; apply Term.Red.refl
-      case lam_congr2 t' r =>
-        constructor; apply (ih1 h).1
-        apply (@ih2 (A::Δ) (preservation_ctx_lift h (Or.inr rfl))).2 _ r
-  case app Γ f A B a B' j1 j2 j3 ih1 ih2 =>
-    apply And.intro
-    case _ =>
-      constructor
-      apply (ih1 h).1; apply (ih2 h).1; apply j3
-    case _ =>
-      intro t' r
-      sorry
-  case econv Γ t A B K j1 j2 j3 ih1 ih2 =>
-    apply And.intro
-    case _ =>
-      constructor
-      apply (ih1 h).1; apply (ih2 h).1; apply j3
-    case _ =>
-      intro t' r
-      sorry
-  case iconv Γ t A B K j1 j2 j3 ih1 ih2 =>
-    apply And.intro
-    case _ =>
-      constructor
-      apply (ih1 h).1; apply (ih2 h).1; apply j3
-    case _ => sorry
+  -- theorem preservation1_term : Γ ⊢ t : A ->
+  --   (∀ n, Γ d@ n -β> Δ d@ n ∨ Γ d@n = Δ d@ n) ->
+  --   Δ ⊢ t : A ∧ (∀ t', t -β> t' -> Δ ⊢ t' : A)
+  -- := by
+  -- intro j h
+  -- induction j generalizing Δ
+  -- case ax Γ f j ih =>
+  --   apply And.intro
+  --   case _ =>
+  --     apply Proof.ax f
+  --     intro x
+  --     cases (h x)
+  --     case _ hx => apply (ih x h).2 _ hx
+  --     case _ hx => rw [<-hx]; apply (ih x h).1
+  --   case _ => intro t' r; cases r
+  -- case var Γ x K j ih =>
+  --   apply And.intro
+  --   case _ =>
+  --     constructor; constructor
+  --     cases (h x)
+  --     case _ hx => apply (ih h).2 _ hx
+  --     case _ hx => rw [<-hx]; apply (ih h).1
+  --     apply (ih h).1
+  --     cases (h x)
+  --     case _ hx =>
+  --       exists (Δ d@ x); apply And.intro
+  --       apply Term.Red.refl; apply Term.RedStar.step; apply hx; apply Term.Red.refl
+  --     case _ hx => rw [hx]; apply Term.RedConv.refl
+  --   case _ => intro t' r; cases r
+  -- case pi Γ A K B j1 j2 ih1 ih2 =>
+  --   apply And.intro
+  --   case _ =>
+  --     constructor
+  --     apply (ih1 h).1
+  --     apply (@ih2 (A::Δ) (preservation_ctx_lift h (Or.inr rfl))).1
+  --   case _ => sorry
+  -- case tpi => sorry
+  -- case lam Γ A B K t j1 j2 ih1 ih2 =>
+  --   apply And.intro
+  --   case _ =>
+  --     constructor
+  --     apply (ih1 h).1
+  --     apply (@ih2 (A::Δ) (preservation_ctx_lift h (Or.inr rfl))).1
+  --   case _ =>
+  --     intro t' r
+  --     cases r
+  --     case lam_congr1 A' r =>
+  --       constructor; constructor
+  --       apply (ih1 h).2 _ (Term.Red.all_congr1 r)
+  --       apply (@ih2 (A'::Δ) (preservation_ctx_lift h (Or.inl r))).1
+  --       apply (ih1 h).1
+  --       exists (.all mf A' B); apply And.intro
+  --       apply Term.Red.refl
+  --       apply Term.Red.congr1 (λ A => .all mf A B) Term.Red.all_congr1
+  --       apply Term.RedStar.step r; apply Term.Red.refl
+  --     case lam_congr2 t' r =>
+  --       constructor; apply (ih1 h).1
+  --       apply (@ih2 (A::Δ) (preservation_ctx_lift h (Or.inr rfl))).2 _ r
+  -- case app Γ f A B a B' j1 j2 j3 ih1 ih2 =>
+  --   apply And.intro
+  --   case _ =>
+  --     constructor
+  --     apply (ih1 h).1; apply (ih2 h).1; apply j3
+  --   case _ =>
+  --     intro t' r
+  --     sorry
+  -- case econv Γ t A B K j1 j2 j3 ih1 ih2 =>
+  --   apply And.intro
+  --   case _ =>
+  --     constructor
+  --     apply (ih1 h).1; apply (ih2 h).1; apply j3
+  --   case _ =>
+  --     intro t' r
+  --     sorry
+  -- case iconv Γ t A B K j1 j2 j3 ih1 ih2 =>
+  --   apply And.intro
+  --   case _ =>
+  --     constructor
+  --     apply (ih1 h).1; apply (ih2 h).1; apply j3
+  --   case _ => sorry
 
   -- theorem preservation_jud : Γ ⊢ t : A ->
   --   (∀ t', t -β> t' -> Γ ⊢ t' : A)
