Fomega/Basic/Weaken.lean
@@ -14,10 +14,6 @@ namespace Fomega.Proof
   cases x <;> simp at *
   case _ x => rw [<-h x]; simp
 
-  -- theorem rename (r : Ren) : Γ ⊢ t : A ->
-  --   (∀ x, [r#r](Γ d@ x) = Δ d@ (r x)) ->
-  --   Δ ⊢ ([r#r]t) : ([r#r]A)
-
   @[simp]
   abbrev idx_ren (r : Ren) : JudgmentIndex v -> JudgmentIndex v :=
     match v with
@@ -37,34 +33,27 @@ namespace Fomega.Proof
   case ax ih =>
     replace ih := ih r h1 h2
     simp at *; constructor; apply ih
-  case var x K T j1 j2 ih =>
+  case var x K T _j1 j2 ih =>
     simp at *; rw [j2, h2 x]; constructor
     rw [<-(h2 x)]; apply ih r h1 h2; rfl
-  case pi Γ' A' K B _j1 _j2 ih1 ih2 =>
+  case pi Γ A K1 K2 B _j1 _j2 ih1 ih2 =>
     simp; constructor
     case _ => apply ih1 r h1 h2
-    case _ =>
-      have lem : ⊢ ([r#r]A' :: Δ) := by constructor; apply h1; apply ih1 r h1 h2
-      replace ih2 := @ih2 ([r#r]A' :: Δ) (Term.Ren.lift r) lem (rename_lift r A' h2)
-      simp at ih2; exact ih2
-  case tpi Γ' A' B _j1 _j2 ih1 ih2 =>
-    simp; constructor
-    case _ => apply ih1 r h1 h2
-    case _ =>
-      have lem : ⊢ ([r#r]A' :: Δ) := by constructor; apply h1; apply ih1 r h1 h2
-      replace ih2 := @ih2 ([r#r]A' :: Δ) (Term.Ren.lift r) lem (rename_lift r A' h2)
-      simp at ih2; exact ih2
-  case lam Γ A B K t j1 j2 ih1 ih2  =>
-    simp; constructor
-    case _ =>
-      have lem : ⊢ ([r#r]A :: Δ) := by
-        constructor; apply h1; replace ih1 := ih1 r h1 h2; simp at ih1
-      replace ih1 := @ih1 ([r#r]A :: Δ) (Term.Ren.lift r) lem (rename_lift r A h2)
-      simp at ih1; exact ih1
     case _ =>
       have lem : ⊢ ([r#r]A :: Δ) := by constructor; apply h1; apply ih1 r h1 h2
       replace ih2 := @ih2 ([r#r]A :: Δ) (Term.Ren.lift r) lem (rename_lift r A h2)
       simp at ih2; exact ih2
+  case lam Γ A K1 K2 B t _j1 _j2 _j3 ih1 ih2 ih3 =>
+    have lem : ⊢ ([r#r]A :: Δ) := by
+      constructor; apply h1; apply ih1 r h1 h2
+    simp; constructor
+    case _ => apply ih1 r h1 h2
+    case _ =>
+      replace ih2 := @ih2 ([r#r]A :: Δ) (Term.Ren.lift r) lem (rename_lift r A h2)
+      simp at ih2; exact ih2
+    case _ =>
+      replace ih3 := @ih3 ([r#r]A :: Δ) (Term.Ren.lift r) lem (rename_lift r A h2)
+      simp at ih3; exact ih3
   case app Γ' f A' B a B' _j1 _j2 j3 ih1 ih2 =>
     simp; constructor
     case _ => apply ih1 r h1 h2
@@ -76,37 +65,13 @@ namespace Fomega.Proof
     case _ => apply ih2 r h1 h2
     case _ => apply RedConv.subst; apply j3
 
-  -- theorem rename_wf (r : Ren) : t ⊢ Γ ->
-  --   (∀ x, [r#r](Γ d@ x) = Δ d@ (r x)) ->
-  --   ([r#r]t) ⊢ Δ
-  -- := by
-  -- intro j h
-  -- induction j generalizing Δ r
-  -- case ax => simp; constructor
-  -- case var j1 _j2 ih =>
-  --   have j2 := rename r j1 h
-  --   simp at *; constructor; rw [h] at j2; exact j2
-  --   replace ih := ih r h; rw [h _] at ih; exact ih
-  -- case pi A Γ B _ _ ih1 ih2 =>
-  --   simp; constructor; apply ih1 r h
-  --   replace ih2 := @ih2 ([r#r]A :: Δ) (Term.Ren.lift r) (rename_lift r A h); simp at ih2
-  --   exact ih2
-  -- case lam A Γ B _ _ ih1 ih2 =>
-  --   simp; constructor; apply ih1 r h
-  --   replace ih2 := @ih2 ([r#r]A :: Δ) (Term.Ren.lift r) (rename_lift r A h); simp at ih2
-  --   exact ih2
-  -- case app _ _ ih1 ih2 =>
-  --   simp; constructor; apply ih1 r h; apply ih2 r h
-  -- case conv _ _ ih1 ih2 =>
-  --   simp; constructor; apply ih1 r h; apply ih2 r h
-
-  -- theorem weaken B : Γ ⊢ t : A -> (B::Γ) ⊢ ([S]t) : ([S]A) := by
-  -- intro j; apply rename; exact j
-  -- case _ => intro x; simp; rw [Term.S_to_rS]; unfold rS; simp
-
-  -- theorem weaken_wf A : t ⊢ Γ -> ([S]t) ⊢ (A::Γ) := by
-  -- intro j; apply rename_wf; exact j
-  -- case _ => intro x; simp; rw [Term.S_to_rS]; unfold rS; simp
-
+  theorem weaken :
+    Γ ⊢ B : .const K ->
+    Γ ⊢ t : A ->
+    (B::Γ) ⊢ ([S]t) : ([S]A)
+  := by
+  intro j1 j2; apply rename _ j2;
+  case _ => constructor; apply judgment_ctx_wf j1; apply j1
+  case _ => intro x; simp; rw [Term.S_to_rS]; unfold rS; simp
 
 namespace Fomega.Proof
