Fomega/Proof.lean
@@ -4,6 +4,10 @@ import Fomega.Ctx
 
 namespace Fomega
 
+  def dom (K1 : Const) : Const -> Const
+  | .type => K1
+  | .kind => .kind
+
   inductive JudgmentVariant : Type
   | prf | wf
 
@@ -26,15 +30,12 @@ namespace Fomega
     T = Γ d@ x ->
     Judgment .prf Γ (.bound K x, T)
   | pi :
-    Judgment .prf Γ (A, .const K) ->
-    Judgment .prf (A::Γ) (B, ★) ->
-    Judgment .prf Γ (.all mf A B, ★)
-  | tpi :
-    Judgment .prf Γ (A, □) ->
-    Judgment .prf (A::Γ) (B, □) ->
-    Judgment .prf Γ (.all mf A B, □)
+    Judgment .prf Γ (A, .const (dom K1 K2)) ->
+    Judgment .prf (A::Γ) (B, .const K2) ->
+    Judgment .prf Γ (.all mf A B, .const K2)
   | lam :
-    Judgment .prf Γ (.all mf A B, .const K) ->
+    Judgment .prf Γ (A, .const (dom K1 K2)) ->
+    Judgment .prf (A::Γ) (B, .const K2) ->
     Judgment .prf (A::Γ) (t, B) ->
     Judgment .prf Γ (.lam mf A t, .all mf A B)
   | app :
@@ -48,52 +49,7 @@ namespace Fomega
     A =β= B ->
     Judgment .prf Γ (t, B)
 
-
   notation:170 Γ:170 " ⊢ " t:170 " : " A:170 => Judgment JudgmentVariant.prf Γ (t, A)
   notation:170 "⊢ " Γ:170 => Judgment JudgmentVariant.wf Γ ()
-
-  @[simp]
-  abbrev all_inversion_idx A B T : JudgmentIndex v :=
-    match v with
-    | .prf => (.all mf A B, T)
-    | .wf => ()
-
-  theorem all_destruct :
-    Γ ⊢ .all mf A B : T ->
-    T =β= .const K ->
-    Γ ⊢ .all mf A B : .const K ∧ (∃ K, Γ ⊢ A : .const K) ∧ (A::Γ) ⊢ B : .const K
-  := by
-  intro j hc
-  generalize tdef : Term.all mf A B = t at *
-  induction j generalizing A B K
-  case ax => simp at tdef
-  case var => simp at tdef
-  case pi Γ' A' K' B' j1 j2 ih1 ih2 =>
-    injection tdef with e1 e2 e3
-    subst e2; subst e3
-    cases K
-    case _ =>
-      apply And.intro; constructor; apply j1; apply j2
-      apply And.intro; exists K'
-      apply j2
-    case _ => exfalso; apply Term.RedConv.type_not_conv_to_kind hc
-  case tpi Γ' A' B' j1 j2 ih1 ih2 =>
-    injection tdef with e1 e2 e3
-    subst e2; subst e3
-    cases K
-    case _ => exfalso; apply Term.RedConv.type_not_conv_to_kind (Term.RedConv.sym hc)
-    case _ =>
-      apply And.intro; constructor; apply j1; apply j2
-      apply And.intro; exists .kind
-      apply j2
-  case lam => simp at tdef
-  case app => simp at tdef
-  case econv Γ t' A' B' _K' h1 _h2 _h3 ih1 _ih2 =>
-    cases t' <;> simp at tdef
-  case iconv Γ t' A' B' _K' h1 _h2 h3 ih1 _ih2 =>
-    cases t' <;> simp at tdef
-    case all m C D =>
-      apply ih1 (Term.RedConv.trans h3 hc)
-      rw [tdef.1, tdef.2.1, tdef.2.2]
 
 end Fomega
